Update Revm v103 host log/selfdestruct slice

RocqOfRust/revm/revm_interpreter/instructions/simulate/host/log.v
@@ -4,16 +4,57 @@ Require Import core.links.array.
 Require Import alloc.links.raw_vec.
 Require Import alloc.vec.links.mod.
 Require Import alloy_primitives.bytes.links.mod.
+Require Import alloy_primitives.bytes.simulate.mod.
 Require Import alloy_primitives.links.aliases.
 Require Import alloy_primitives.log.links.mod.
+Require Import core.ops.simulate.deref.
 Require Import revm.revm_context_interface.links.host.
 Require Import revm.revm_context_interface.links.journaled_state.
 Require Import revm.revm_context_interface.simulate.host.
+Require Import revm.revm_interpreter.gas.simulate.calc.
 Require Import revm.revm_interpreter.instructions.links.host.log.
 Require Import revm.revm_interpreter.instructions.simulate.macros.
 Require Import revm.revm_interpreter.links.interpreter.
+Require Import revm.revm_interpreter.links.instruction_context.
 Require Import revm.revm_interpreter.links.interpreter_types.
 Require Import revm.revm_interpreter.simulate.interpreter_types.
+
+Definition topics_from_array
+    (N : usize)
+    (topics : array.t aliases.U256.t N) :
+    Vec.t aliases.U256.t Global.t :=
+  {|
+    Vec.buf := {| RawVec.value := ArrayPairs.to_list topics.(array.value) |};
+    Vec.len := N;
+  |}.
+
+Definition finish_log
+    (N : usize)
+    {WIRE H : Set} `{Link WIRE} `{Link H}
+    {WIRE_types : InterpreterTypes.Types.t} `{InterpreterTypes.Types.AreLinks WIRE_types}
+    {IInterpreterTypes : InterpreterTypes.C WIRE_types}
+    {H_types : Host.Types.t} `{Host.Types.AreLinks H_types}
+    {IHost : Host.C H H_types}
+    (interpreter : Interpreter.t WIRE WIRE_types)
+    (host : H)
+    (data : alloy_primitives.bytes.links.mod.Bytes.t) :
+    Interpreter.t WIRE WIRE_types * H :=
+  popn_macro interpreter N
+    (fun interpreter => (interpreter, host)) (fun topics interpreter =>
+  let target :=
+    IInterpreterTypes.(InterpreterTypes.InputsTrait_for_Input).(InputTraits.target_address)
+      interpreter.(Interpreter.input) in
+  let topics := topics_from_array N topics in
+  let log' : Log.t LogData.t := {|
+    Log.address := target;
+    Log.data := {|
+      LogData.topics := topics;
+      LogData.data := data;
+    |};
+  |} in
+  let host := IHost.(Host.log) host log' in
+  (interpreter, host)
+  ).
 
 Definition log
     (N : usize)
@@ -25,27 +66,36 @@ Definition log
     (interpreter : Interpreter.t WIRE WIRE_types)
     (host : H) :
     Interpreter.t WIRE WIRE_types * H :=
-  popn_macro interpreter 2 (fun interpreter => (interpreter, host)) (fun _arr interpreter =>
-    let target :=
-      IInterpreterTypes.(InterpreterTypes.InputsTrait_for_Input).(InputTraits.target_address)
-        interpreter.(Interpreter.input) in
-    let topics : Vec.t aliases.U256.t Global.t := {|
-      Vec.buf := {| RawVec.value := [] |};
-      Vec.len := 0;
-    |} in
-    let data : alloy_primitives.bytes.links.mod.Bytes.t := {|
-      alloy_primitives.bytes.links.mod.Bytes.value := {| bytes.Bytes.value := [] |};
-    |} in
-    let log' : Log.t LogData.t := {|
-      Log.address := target;
-      Log.data := {|
-        LogData.topics := topics;
-        LogData.data := data;
-      |};
-    |} in
-    let host := IHost.(Host.log) host log' in
-    (interpreter, host)
-  ).
+  require_non_staticcall_macro interpreter
+    (fun interpreter => (interpreter, host)) (fun interpreter =>
+  popn_macro interpreter 2 (fun interpreter => (interpreter, host)) (fun arr interpreter =>
+    let '⟬ offset; len ⟭ := arr.(array.value) in
+    as_usize_or_fail_macro interpreter len None
+      (fun interpreter => (interpreter, host)) (fun len interpreter =>
+    gas_or_fail_macro interpreter
+      (calc.log_cost (M.cast_integer IntegerKind.U8 N) (M.cast_integer IntegerKind.U64 len))
+      (fun interpreter => (interpreter, host)) (fun interpreter =>
+    if i[len] =? 0 then
+      finish_log N interpreter host Impl_Bytes.new
+    else
+      as_usize_or_fail_macro interpreter offset None
+        (fun interpreter => (interpreter, host)) (fun offset interpreter =>
+      resize_memory_macro interpreter offset len
+        (fun interpreter => (interpreter, host)) (fun interpreter =>
+        let slice :=
+          IInterpreterTypes.(InterpreterTypes.MemoryTrait_for_Memory).(MemoryTrait.slice_len)
+            interpreter.(Interpreter.memory)
+            offset
+            len in
+        let data :=
+          IInterpreterTypes
+            .(InterpreterTypes.MemoryTrait_for_Memory)
+            .(MemoryTrait.Deref_for_Synthetic)
+            .(Deref.deref)
+            .(RefStub.projection)
+            slice in
+        finish_log N interpreter host (Impl_Bytes.copy_from_slice data))
+  ))))).
 
 Lemma log_eq
     (N : usize)
@@ -63,10 +113,14 @@ Lemma log_eq
     (host : H) :
   let ref_interpreter := make_ref 0 in
   let ref_host := make_ref (A := H) 1 in
+  let context := {|
+    instruction_context.InstructionContext.interpreter := ref_interpreter;
+    instruction_context.InstructionContext.host := ref_host;
+  |} in
   let result := log N interpreter host in
   {{
     SimulateM.eval_f
-      (run_log (N := N) run_InterpreterTypes_for_WIRE run_Host_for_H ref_interpreter ref_host)
+      (run_log (N := N) run_InterpreterTypes_for_WIRE run_Host_for_H context)
       [interpreter; host]%stack 🌲
     (
       Output.Success tt,
