RocqOfRust/revm/revm_interpreter/instructions/links/host/log.v
@@ -22,6 +22,7 @@ Require Import revm.revm_interpreter.instructions.host.
 Require Import revm.revm_interpreter.instructions.links.utility.
 Require Import revm.revm_interpreter.interpreter.links.shared_memory.
 Require Import revm.revm_interpreter.links.gas.
+Require Import revm.revm_interpreter.links.instruction_context.
 Require Import revm.revm_interpreter.links.instruction_result.
 Require Import revm.revm_interpreter.links.interpreter.
 Require Import revm.revm_interpreter.links.interpreter_types.
@@ -33,8 +34,7 @@ Require Import ruint.links.lib.
 
 (*
 pub fn log<const N: usize, H: Host + ?Sized>(
-    interpreter: &mut Interpreter<impl InterpreterTypes>,
-    host: &mut H,
+    context: InstructionContext<'_, H, impl InterpreterTypes>,
 )
 *)
 Instance run_log
@@ -44,31 +44,70 @@ Instance run_log
     {H_types : Host.Types.t} `{Host.Types.AreLinks H_types}
     (run_InterpreterTypes_for_WIRE : InterpreterTypes.Run WIRE WIRE_types)
     (run_Host_for_H : Host.Run H H_types)
-    (interpreter : '&mut (Interpreter.t WIRE WIRE_types))
-    (host : '&mut H) :
+    (context : InstructionContext.t H WIRE WIRE_types) :
   Run.Trait
-    instructions.host.log [ φ N ] [ Φ H; Φ WIRE ] [ φ interpreter; φ host ]
+    instructions.host.log [ φ N ] [ Φ H; Φ WIRE ] [ φ context ]
     unit.
 Proof.
   constructor.
+  pose proof run_InterpreterTypes_for_WIRE as run_InterpreterTypes_for_WIRE_copy.
   destruct run_InterpreterTypes_for_WIRE.
   destruct run_StackTrait_for_Stack.
+  pose proof run_MemoryTrait_for_Memory as run_MemoryTrait_for_Memory_copy.
   destruct run_MemoryTrait_for_Memory.
   destruct run_RuntimeFlag_for_RuntimeFlag.
   destruct run_InputsTrait_for_Input.
   destruct run_LoopControl_for_Control.
+  destruct run_LoopControl_for_Bytecode.
   destruct run_Host_for_H.
   destruct (Impl_AsRef_for_Slice.run u8).
   destruct run_Deref_for_Synthetic.
   destruct (
+    let U256 := Uint.t {| Integer.value := 256 |} {| Integer.value := 4 |} in
     let B := FixedBytes.t {| Integer.value := 32 |} in
-    let I := IntoIter.t aliases.U256.t N in
-    let F := Function1.t aliases.U256.t B in
+    let I := IntoIter.t U256 N in
+    let F := Function1.t U256 B in
     Impl_Iterator_for_Map.run B I F
   ).
-  destruct (array.links.iter.Impl_Iterator_for_IntoIter.run aliases.U256.t N).
-  destruct (Impl_IntoIterator_for_Array.run aliases.U256.t N).
+  destruct (
+    array.links.iter.Impl_Iterator_for_IntoIter.run
+      (Uint.t {| Integer.value := 256 |} {| Integer.value := 4 |})
+      N
+  ).
+  destruct (
+    Impl_IntoIterator_for_Array.run
+      (Uint.t {| Integer.value := 256 |} {| Integer.value := 4 |})
+      N
+  ).
   destruct Impl_From_U256_for_FixedBytes_32.run.
   run_symbolic.
+  all: try eapply (@Impl_Interpreter.run_halt
+    WIRE _ WIRE_types _ run_InterpreterTypes_for_WIRE_copy).
+  all: try eapply (@Impl_Interpreter.run_halt_oog
+    WIRE _ WIRE_types _ run_InterpreterTypes_for_WIRE_copy).
+  all: try eapply (@Impl_Interpreter.run_halt_memory_oog
+    WIRE _ WIRE_types _ run_InterpreterTypes_for_WIRE_copy).
+  all: try eapply (@Impl_Interpreter.run_halt_underflow
+    WIRE _ WIRE_types _ run_InterpreterTypes_for_WIRE_copy).
+  all: try eapply run_resize_memory.
+  all: try exact run_MemoryTrait_for_Memory_copy.
+  all: try eapply method_map0.(iterator.Iterator.run_map).
+  progress change
+    (Value.Closure (existS (_, _) (method_from.(From.from) [] [])))
+    with (φ (Function1.of_run method_from.(From.run_from))).
+  destruct method_map0 as [? ? run_map].
+  cbn in *.
+  epose proof (
+    run_map' :=
+      run_map
+        (FixedBytes.t {| Integer.value := 32 |})
+        (Function1.t
+          aliases.U256.t
+          (FixedBytes.t {| Integer.value := 32 |}))
+        _ _
+        value_inter2
+        (Function1.of_run method_from.(From.run_from))
+  ).
+  exact run_map'.
 Defined.
 Global Opaque run_log.
